`continue` -> `ctinue`

src/lowparse/LowParse.Low.Base.fst
@@ -2477,9 +2477,9 @@ let list_fold_left_gen
       valid_list p h sl pos2 pos' /\
       inv h (contents_list p h sl pos pos1) (contents p h sl pos1 :: contents_list p h sl pos2 pos') pos1
     ))
-    (ensures (fun h continue h' ->
+    (ensures (fun h ctinue h' ->
       B.modifies (Ghost.reveal l) h h' /\
-      (if continue then inv h' (contents_list p h sl pos pos1 `L.append` [contents p h sl pos1]) (contents_list p h sl pos2 pos') pos2 else post_interrupt h')
+      (if ctinue then inv h' (contents_list p h sl pos pos1 `L.append` [contents p h sl pos1]) (contents_list p h sl pos2 pos') pos2 else post_interrupt h')
     ))
   ))
 : HST.Stack bool
@@ -2496,18 +2496,18 @@ let list_fold_left_gen
   let h1 = HST.get () in
   //B.fresh_frame_modifies h0 h1;
   let bpos : B.pointer U32.t = B.alloca pos 1ul in
-  let bcontinue : B.pointer bool = B.alloca true 1ul in
+  let bctinue : B.pointer bool = B.alloca true 1ul in
   let btest: B.pointer bool = B.alloca (pos `U32.lt` pos') 1ul in
   let h2 = HST.get () in
   let test_pre (h: HS.mem) : GTot Type0 =
-    B.live h bpos /\ B.live h bcontinue /\ B.live h btest /\ (
+    B.live h bpos /\ B.live h bctinue /\ B.live h btest /\ (
     let pos1 = Seq.index (B.as_seq h bpos) 0 in
-    let continue = Seq.index (B.as_seq h bcontinue) 0 in
+    let ctinue = Seq.index (B.as_seq h bctinue) 0 in
     valid_list p h0 sl pos pos1 /\
     valid_list p h0 sl pos1 pos' /\
     B.modifies (Ghost.reveal l `B.loc_union` B.loc_region_only true (HS.get_tip h1)) h2 h /\
-    Seq.index (B.as_seq h btest) 0 == ((U32.v (Seq.index (B.as_seq h bpos) 0) < U32.v pos') && Seq.index (B.as_seq h bcontinue) 0) /\
-    (if continue then inv h (contents_list p h0 sl pos pos1) (contents_list p h0 sl pos1 pos') pos1 else post_interrupt h)
+    Seq.index (B.as_seq h btest) 0 == ((U32.v (Seq.index (B.as_seq h bpos) 0) < U32.v pos') && Seq.index (B.as_seq h bctinue) 0) /\
+    (if ctinue then inv h (contents_list p h0 sl pos pos1) (contents_list p h0 sl pos1 pos') pos1 else post_interrupt h)
   )
   in
   let test_post (cond: bool) (h: HS.mem) : GTot Type0 =
@@ -2532,7 +2532,7 @@ let list_fold_left_gen
       let pos2 = j sl pos1 in
       let h52 = HST.get () in
       inv_frame h51 (contents_list p h0 sl pos pos1) (contents_list p h1 sl pos1 pos') pos1 h52;
-      let continue = body pos1 pos2 in
+      let ctinue = body pos1 pos2 in
       let h53 = HST.get () in
       //assert (B.loc_includes (loc_slice_from_to sl pos pos') (loc_slice_from_to sl pos1 pos2));
       //assert (B.loc_includes (loc_slice_from_to sl pos pos') (loc_slice_from_to sl pos2 pos'));
@@ -2541,12 +2541,12 @@ let list_fold_left_gen
       valid_pos_frame_strong p h0 sl pos1 pos2 (Ghost.reveal l) h53;
       valid_list_snoc p h0 sl pos pos1;
       B.upd bpos 0ul pos2;
-      B.upd bcontinue 0ul continue;
-      B.upd btest 0ul ((pos2 `U32.lt` pos') && continue);
+      B.upd bctinue 0ul ctinue;
+      B.upd btest 0ul ((pos2 `U32.lt` pos') && ctinue);
       let h54 = HST.get () in
       [@inline_let]
       let _ =
-        if continue
+        if ctinue
         then inv_frame h53 (contents_list p h0 sl pos pos2) (contents_list p h0 sl pos2 pos') pos2 h54
         else post_interrupt_frame h53 h54
       in
@@ -2560,7 +2560,7 @@ let list_fold_left_gen
     while_body
     ;
   valid_list_nil p h0 sl pos';
-  let res = B.index bcontinue 0ul in
+  let res = B.index bctinue 0ul in
   let h3 = HST.get () in
   HST.pop_frame ();
   let h4 = HST.get () in
